Simplify `Strategy` with `FinalB` and `TransB`

code/verification/Trans.v
@@ -33,16 +33,74 @@ Inductive Trans: relation State :=
   NoDecisions n ->
   Trans (state (m ++d l ++a n) f Hwf) (state (m ++p ¬l) f Hwf').
 
+Inductive TransB: relation State :=
+(* Fail if all literals are assigned and there is a conflict. *)
+| tb_fail (m: PA) (f: CNF) (c: Clause) (Hwf: WellFormed m f):
+  In c f ->
+  Conflicting m c ->
+  NoDecisions m ->
+  TransB (state m f Hwf) fail
+(* Arbitrarily set an unassigned literal in the formula to true. *)
+| tb_decide (m: PA) (f: CNF) (c: Clause) (l: Lit) (Hwf: WellFormed m f) (Hwf': WellFormed (m ++d l) f):
+  In l c \/ In (¬l) c ->
+  In c f ->
+  Undef m l ->
+  TransB (state m f Hwf) (state (m ++d l) f Hwf')
+(* Backtrack by flipping the most recent decision literal. *)
+| tb_backtrack (m n: PA) (f: CNF) (c: Clause) (l: Lit) (Hwf: WellFormed (m ++d l ++a n) f) (Hwf': WellFormed (m ++p ¬l) f):
+  In c f ->
+  Conflicting (m ++d l ++a n) c ->
+  NoDecisions n ->
+  TransB (state (m ++d l ++a n) f Hwf) (state (m ++p ¬l) f Hwf').
+
 (* The following is the reflexive-transitive closure of `==>`. *)
 Definition Derivation: relation State := clos_refl_trans State Trans.
 
 Declare Scope trans_scope.
 Infix "==>" := Trans (at level 70): trans_scope.
+Infix "==>b" := TransB (at level 70): trans_scope.
 Infix "==>*" := Derivation (at level 70): trans_scope.
 Open Scope trans_scope.
 
 (* A state is final if there are no states that follow from it by `==>`. *)
 Definition Final (s: State): Prop := ~ exists (s': State), s ==> s'.
+Definition FinalB (s: State): Prop := ~ exists (s': State), s ==>b s'.
+
+Lemma final__final_b: forall (s: State), Final s <-> FinalB s.
+Proof.
+  split.
+  - unfold FinalB. unfold not. intros H [s' Htrans]. apply H. inversion Htrans as
+    [
+      m f c_conflict Hwf' Hc_in_f Hconflict Hno_dec |
+      m f c_decide l_decide Hwf Hwf' Hx_in_c Hc_in_f Hundef |
+      m_split n_split f c_conflict l_split Hwf Hwf' Hc_in_f Hconflict Hno_dec
+    ]; subst s; subst s'.
+    + exists fail. now apply (t_fail _ _ c_conflict).
+    + exists (state (m ++d l_decide) f Hwf'). now apply (t_decide _ _ c_decide).
+    + exists (state (m_split ++p (¬l_split)) f Hwf'). now apply (t_backtrack _ _ _ c_conflict).
+  - unfold Final. unfold not. intros H [s' Htrans]. apply H. inversion Htrans as
+    [
+      m f c_conflict Hwf' Hc_in_f Hconflict Hno_dec |
+      m f c_unit l_unit Hwf Hwf' Hl_in_c Hc_in_f Hconflict Hundef |
+      m f c_decide l_decide Hwf Hwf' Hx_in_c Hc_in_f Hundef |
+      m_split n_split f c_conflict l_split Hwf Hwf' Hc_in_f Hconflict Hno_dec
+    ]; subst s; subst s'.
+    + exists fail. now apply (tb_fail _ _ c_conflict).
+    + assert (Hwf'': WellFormed (m ++d l_unit) f).
+      * unfold WellFormed. split.
+        -- apply nodup_cons.
+          ++ apply Hwf.
+          ++ assumption.
+        -- apply bounded_cons.
+          ++ apply Hwf.
+          ++ apply l_in_f_true_iff. exists c_unit. intuition.
+      * exists (state (m ++d l_unit) f Hwf''). apply (tb_decide _ _ c_unit).
+        -- intuition.
+        -- assumption.
+        -- assumption.
+    + exists (state (m ++d l_decide) f Hwf'). now apply (tb_decide _ _ c_decide).
+    + exists (state (m_split ++p (¬l_split)) f Hwf'). now apply (tb_backtrack _ _ _ c_conflict).
+Qed.
 
 Lemma fail_final: Final fail.
 Proof. unfold Final. unfold not. intros. inversion H. inversion H0. Qed.
